src/Language/PlutusIR/Semantics/Static/Implementations/Named.v
@@ -155,7 +155,18 @@ Definition binds (b : Binding) : Context :=
     matchB :T: constrBs_ctx ++ (dataB :K: nil)
   end.
 
-  (** ** Types of builtin-functions *)
+(** ** Kinds of builtin types *)
+Definition lookupBuiltinKind (u : DefaultUni) : Kind := 
+  match u with
+  | DefaultUniInteger    => Kind_Base
+  | DefaultUniByteString => Kind_Base
+  | DefaultUniString     => Kind_Base
+  | DefaultUniChar       => Kind_Base
+  | DefaultUniUnit       => Kind_Base
+  | DefaultUniBool       => Kind_Base
+  end.
+
+(** ** Types of builtin functions *)
 Definition lookupBuiltinTy (f : DefaultFun) : Ty :=
   let Ty_Int := Ty_Builtin (Some (TypeIn DefaultUniInteger)) in
   let Ty_Bool := Ty_Builtin (Some (TypeIn DefaultUniBool)) in
@@ -228,26 +239,30 @@ Definition fromDecl (tvd : tvdecl tyname) : Context :=
     
 Definition unwrapIFix (F : Ty) (X : binderTyname) (K : Kind) (T : Ty) : Ty := (Ty_App (Ty_App F (Ty_Lam X K (Ty_IFix F (Ty_Var X)))) T).
 
-Definition has_kind__named : Context -> Ty -> Kind -> Prop := has_kind tyname binderTyname Context lookupK extendK.
+Definition has_kind__named : Context -> Ty -> Kind -> Prop := has_kind tyname binderTyname Context lookupK extendK lookupBuiltinKind.
 
-Notation "ctx '|-*' T ':' K" := (has_kind tyname binderTyname Context lookupK extendK ctx T K) (at level 40, T at level 0, K at level 0).
+Notation "ctx '|-*' T ':' K" := (has_kind tyname binderTyname Context lookupK extendK lookupBuiltinKind ctx T K) (at level 40, T at level 0, K at level 0).
 
-Definition has_type__named : Context -> Term -> Ty -> Prop := has_type name tyname binderName binderTyname Context lookupT lookupK extendT extendK flatten append binds fromDecl lookupBuiltinTy substituteT listOfArgumentTypes unwrapIFix.
+Definition has_type__named : Context -> Term -> Ty -> Prop := has_type name tyname binderName binderTyname Context lookupT lookupK extendT extendK flatten append binds fromDecl lookupBuiltinKind lookupBuiltinTy substituteT listOfArgumentTypes unwrapIFix.
 
-Notation "ctx '|-+' tm ':' T" := (has_type name tyname binderName binderTyname Context lookupT lookupK extendT extendK flatten append binds fromDecl lookupBuiltinTy substituteT listOfArgumentTypes unwrapIFix ctx tm T) (at level 40, tm at level 0, T at level 0).
+Notation "ctx '|-+' tm ':' T" := (has_type name tyname binderName binderTyname Context lookupT lookupK extendT extendK flatten append binds fromDecl lookupBuiltinKind lookupBuiltinTy substituteT listOfArgumentTypes unwrapIFix ctx tm T) (at level 40, tm at level 0, T at level 0).
 
 Definition EqT__named : Ty -> Ty -> Prop := EqT tyname binderTyname substituteT.
 
 Notation "T1 '=b' T2" := (EqT tyname binderTyname substituteT T1 T2) (at level 40).
 
-Definition constructor_well_formed__named : Context -> constructor -> Prop := constructor_well_formed name tyname binderName binderTyname Context lookupT lookupK extendT extendK flatten append binds fromDecl lookupBuiltinTy substituteT listOfArgumentTypes unwrapIFix.
+Definition constructor_well_formed__named : Context -> constructor -> Prop := constructor_well_formed name tyname binderName binderTyname Context lookupT lookupK extendT extendK flatten append binds fromDecl lookupBuiltinKind lookupBuiltinTy substituteT listOfArgumentTypes unwrapIFix.
 
-Notation "ctx '|-ok_c' c" := (constructor_well_formed name tyname binderName binderTyname Context lookupT lookupK extendT extendK flatten append binds fromDecl lookupBuiltinTy substituteT listOfArgumentTypes unwrapIFix ctx c) (at level 40, c at level 0).
+Notation "ctx '|-ok_c' c" := (constructor_well_formed name tyname binderName binderTyname Context lookupT lookupK extendT extendK flatten append binds fromDecl lookupBuiltinKind lookupBuiltinTy substituteT listOfArgumentTypes unwrapIFix ctx c) (at level 40, c at level 0).
 
-Definition bindings_well_formed__named : Context -> list Binding -> Prop := bindings_well_formed name tyname binderName binderTyname Context lookupT lookupK extendT extendK flatten append binds fromDecl lookupBuiltinTy substituteT listOfArgumentTypes unwrapIFix.
+Definition bindings_well_formed_nonrec__named : Context -> list Binding -> Prop := bindings_well_formed_nonrec name tyname binderName binderTyname Context lookupT lookupK extendT extendK flatten append binds fromDecl lookupBuiltinKind lookupBuiltinTy substituteT listOfArgumentTypes unwrapIFix.
 
-Notation "ctx '|-oks' bs" := (bindings_well_formed name tyname binderName binderTyname Context lookupT lookupK extendT extendK flatten append binds fromDecl lookupBuiltinTy substituteT listOfArgumentTypes unwrapIFix ctx bs) (at level 40, bs at level 0).
+Notation "ctx '|-oks_nr' bs" := (bindings_well_formed_nonrec name tyname binderName binderTyname Context lookupT lookupK extendT extendK flatten append binds fromDecl lookupBuiltinKind lookupBuiltinTy substituteT listOfArgumentTypes unwrapIFix ctx bs) (at level 40, bs at level 0).
 
-Definition binding_well_formed__named : Context -> Binding -> Prop := binding_well_formed name tyname binderName binderTyname Context lookupT lookupK extendT extendK flatten append binds fromDecl lookupBuiltinTy substituteT listOfArgumentTypes unwrapIFix.
+Definition bindings_well_formed_rec__named : Context -> list Binding -> Prop := bindings_well_formed_rec name tyname binderName binderTyname Context lookupT lookupK extendT extendK flatten append binds fromDecl lookupBuiltinKind lookupBuiltinTy substituteT listOfArgumentTypes unwrapIFix.
 
-Notation "ctx '|-ok' tm" := (binding_well_formed name tyname binderName binderTyname Context lookupT lookupK extendT extendK flatten append binds fromDecl lookupBuiltinTy substituteT listOfArgumentTypes unwrapIFix ctx tm) (at level 40, tm at level 0).
+Notation "ctx '|-oks_r' bs" := (bindings_well_formed_rec name tyname binderName binderTyname Context lookupT lookupK extendT extendK flatten append binds fromDecl lookupBuiltinKind lookupBuiltinTy substituteT listOfArgumentTypes unwrapIFix ctx bs) (at level 40, bs at level 0).
+
+Definition binding_well_formed__named : Context -> Binding -> Prop := binding_well_formed name tyname binderName binderTyname Context lookupT lookupK extendT extendK flatten append binds fromDecl lookupBuiltinKind lookupBuiltinTy substituteT listOfArgumentTypes unwrapIFix.
+
+Notation "ctx '|-ok' tm" := (binding_well_formed name tyname binderName binderTyname Context lookupT lookupK extendT extendK flatten append binds fromDecl lookupBuiltinKind lookupBuiltinTy substituteT listOfArgumentTypes unwrapIFix ctx tm) (at level 40, tm at level 0).
